proof/invariant-abstract/RISCV64/ArchDetSchedAux_AI.thy
@@ -24,8 +24,8 @@ lemma set_pt_ntfns_of[wp]:
   "set_pt ptr pt \<lbrace>\<lambda>s. P (ntfns_of s)\<rbrace>"
   by (set_object_easy_cases def: set_pt_def)
 
-lemma set_pt_prios_of[wp]:
-  "set_pt ptr pt \<lbrace>\<lambda>s. P (prios_of s)\<rbrace>"
+lemma set_pt_tcbs_of[wp]:
+  "set_pt ptr pt \<lbrace>\<lambda>s. P (tcbs_of s)\<rbrace>"
   by (set_object_easy_cases def: set_pt_def)
 
 lemma set_pt_valid_sched_pred[wp]:
